trunk/coq/playground/himp/kstyle.v
@@ -12,6 +12,7 @@ Require Import domains.
 Notation "'□' '+' e" := (Fplusl e) (at level 50) : k_scope.
 Notation "e '+' '□'" := (Fplusr e) (at level 50) : k_scope.
  *)
+
 Notation FreezeL f e := (KFreezeE (fun x => f x e)).
 Notation FreezeR f e := (KFreezeE (fun x => f e x)).
 
@@ -21,11 +22,13 @@ Notation "'□' '-' e" := (FreezeL EMinus e) (at level 50) : k_scope.
 Notation "e '-' '□'" := (FreezeR EMinus e) (at level 50) : k_scope.
 Notation "'□/' e" := (FreezeL EDiv e) (at level 50): k_scope.
 Notation "e '/□'" := (FreezeR EDiv e) (at level 50): k_scope.
-Notation "'□' '<=' e" := (FreezeL BLe e) (at level 70): k_scope.
-Notation "i '<=' '□'" := (FreezeR BLe (ECon i)) (at level 70): k_scope.
-Notation "'□' '&&' e" := (KFreezeB (fun l => BAnd l e)) (at level 50): k_scope.
+Notation "'□<=' e" := (FreezeL BLe e) (at level 70): k_scope.
+Notation "i '<=□'" := (FreezeR BLe (ECon i)) (at level 70): k_scope.
+Notation "'□==' e" := (FreezeL BEq e) (at level 70): k_scope.
+Notation "i '==□'" := (FreezeR BEq (ECon i)) (at level 70): k_scope.
+Notation "'□&&' e" := (KFreezeB (fun l => BAnd l e)) (at level 50): k_scope.
 Notation "v ':=□'" := (KFreezeE (fun e => SAssign v e)) (at level 70): k_scope.
-Notation "'if□then' s1 'else' s2" := (Fif s1 s2) (at level 20): k_scope.
+Notation "'if□then' s1 'else' s2" := (KFreezeB (fun b => SIf b s1 s2)) (at level 20): k_scope.
 
 Delimit Scope k_scope with K.
 Open Scope k_scope.
@@ -33,7 +36,6 @@ Open Scope k_scope.
 Coercion KExp : Exp >-> kitem.
 Coercion KBExp : BExp >-> kitem.
 Coercion KStmt : Stmt >-> kitem.
-Coercion KFreezer : freezer >-> kitem.
 
 Set Implicit Arguments.
 
@@ -47,15 +49,21 @@ Notation heat_step step cool hot ctx :=
 Notation cool_step step hot ctx cool :=
   (forall rest, exp_step step (kra hot (kra ctx rest)) (kra cool rest)).
 
-Generalizable Variables rest env erest henv lenv x y i j v r e b s.
+Generalizable Variables rest env erest henv hrest lenv x y i j v r e b s.
 Inductive kstep : kcfg -> kcfg -> Prop :=
   (* evaluation rules *)
   | k_lookup : `(env ~= (x |-> i :* erest) ->
                  kstep (KCfg (kra (EVar x) rest) env henv lenv)
                        (KCfg (kra (ECon i) rest) (x |-> i :* erest) henv lenv))
+  | k_load : `(henv ~= (i |-> j :* hrest) ->
+                 kstep (KCfg (kra (ELoad (ECon i)) rest) env henv lenv)
+                       (KCfg (kra (ECon j) rest) env henv lenv))
   | k_assign : `(env ~= (x |-> v :* erest) ->
                  kstep (KCfg (kra (SAssign x (ECon i)) rest) env henv lenv)
-                       (KCfg (kra Skip rest) (x |-> i :* erest) henv lenv))
+                       (KCfg             rest (x |-> i :* erest) henv lenv))
+  | k_hassign : `(henv ~= (i |-> v :* hrest) ->
+                 kstep (KCfg (kra (HAssign (ECon i) (ECon j)) rest) env henv lenv)
+                       (KCfg                     rest env (i |-> j :* hrest) lenv))
   | k_jump : `(forall l,
                  lenv ~= (l |-> s :* erest) ->
                  kstep (KCfg (kra (Jump l) rest) env henv lenv)
@@ -69,6 +77,9 @@ Inductive kstep : kcfg -> kcfg -> Prop :=
                                (ECon (Zdiv i j)))
   | k_le : `(exp1_step kstep (BLe (ECon i) (ECon j))
                              (BCon (Zle_bool i j)))
+  | k_eq : `(exp1_step kstep (BEq (ECon i) (ECon j))
+                             (BCon (i =? j)%Z))
+  | k_not : `(exp1_step kstep (BNot (BCon b)) (BCon (negb b)))
   | k_and_t : `(exp1_step kstep (BAnd (BCon true) b)
                                 b)
   | k_and_f : `(exp1_step kstep (BAnd (BCon false) b)
@@ -84,47 +95,33 @@ Inductive kstep : kcfg -> kcfg -> Prop :=
   (* heating and cooling *)
   | k_cool_e : `(cool_step kstep (ECon i) (KFreezeE e) (e (ECon i)))
   | k_cool_b : `(cool_step kstep (BCon b) (KFreezeB e) (e (BCon b)))
+  (* unary *)
+  | k_heat_load : `(isEVal e = false -> heat_step kstep (ELoad e) e (KFreezeE ELoad))
   (* plus *)
   | k_heat_plus_l : `(isEVal e = false ->  heat_step kstep (EPlus e e2) e  (□ + e2))
   | k_heat_plus_r : `(isEVal e2 = false -> heat_step kstep (EPlus e e2) e2 (e + □))
-(*
-  | k_cool_plus_l : `(cool_step kstep (ECon i) (□ + e) (EPlus (ECon i) e))
-  | k_cool_plus_r : `(cool_step kstep (ECon i) (e + □) (EPlus e (ECon i)))
- *)
   (* minus *)
   | k_heat_minus_l : `(isEVal e = false ->  heat_step kstep (EMinus e e2) e  (□ - e2))
   | k_heat_minus_r : `(isEVal e2 = false -> heat_step kstep (EMinus e e2) e2 (e - □))
-(*
-  | k_cool_minus_l : `(cool_step kstep (ECon i) (□ - e) (EMinus (ECon i) e))
-  | k_cool_minus_r : `(cool_step kstep (ECon i) (e - □) (EMinus e (ECon i)))
-*)
   (* div *)
   | k_heat_div_l : `(isEVal e = false ->  heat_step kstep (EDiv e e2) e (□/ e2))
   | k_heat_div_r : `(isEVal e2 = false -> heat_step kstep (EDiv e e2) e2 (e /□))
-(*
-  | k_cool_div_l : `(cool_step kstep (ECon i) (□/ e) (EDiv (ECon i) e))
-  | k_cool_div_r : `(cool_step kstep (ECon i) (e /□) (EDiv e (ECon i)))
- *)
   (* le is seqstrict *)
-  | k_heat_le_l : `(isEVal e = false ->  heat_step kstep (BLe e e2) e (□ <= e2))
-  | k_heat_le_r : `(isEVal e2 = false -> heat_step kstep (BLe (ECon i) e2) e2 (i <= □))
-(*
-  | k_cool_le_l : `(cool_step kstep (ECon i) (□ <= e) (BLe (ECon i) e))
-  | k_cool_le_r : `(cool_step kstep (ECon j) (i <= □) (BLe (ECon i) (ECon j)))
- *)
+  | k_heat_le_l : `(isEVal e = false ->  heat_step kstep (BLe e e2) e (□<= e2))
+  | k_heat_le_r : `(isEVal e2 = false -> heat_step kstep (BLe (ECon i) e2) e2 (i <=□))
+  (* eq is seqstrict *)
+  | k_heat_eq_l : `(isEVal e = false ->  heat_step kstep (BEq e e2) e (□== e2))
+  | k_heat_eq_r : `(isEVal e2 = false -> heat_step kstep (BEq (ECon i) e2) e2 (i ==□))
   (* and is only strict in left argument *)
-  | k_heat_and : `(isBool b1 = false -> heat_step kstep (BAnd b1 b2) b1 (□ && b2))
-(*
-  | k_cool_and : `(cool_step kstep (BCon b) (□ && b2) (BAnd (BCon b) b2))
- *)
+  | k_heat_not : `(isBool b = false -> heat_step kstep (BNot b) b (KFreezeB BNot))
+  | k_heat_and : `(isBool b1 = false -> heat_step kstep (BAnd b1 b2) b1 (□&& b2))
   (* assign *)
   | k_heat_assign : `(isEVal e = false -> heat_step kstep (SAssign x e) e (x :=□))
-(*
-  | k_cool_assign : `(cool_step kstep (ECon i) (x :=□) (SAssign x (ECon i)))
- *)
+  (* hassign *)
+  | k_heat_hassign_l : `(isEVal e  = false -> heat_step kstep (HAssign e e2) e  (FreezeL HAssign e2))
+  | k_heat_hassign_r : `(isEVal e2 = false -> heat_step kstep (HAssign e e2) e2 (FreezeR HAssign e))
   (* if *)
   | k_heat_if : `(isBool b = false -> heat_step kstep (SIf b s1 s2) b (if□then s1 else s2))
-  | k_cool_if : `(cool_step kstep (BCon b) (if□then s1 else s2) (SIf (BCon b) s1 s2))
   (* seq *)
   | k_heat_seq : `(heat_step kstep (Seq s1 s2) s1 s2)
   .
@@ -166,6 +163,18 @@ Add Parametric Relation : kcfg kequiv
   symmetry proved by kequiv_sym
   transitivity proved by kequiv_trans
   as kequiv_rel.
+
+Lemma kstep_equiv : forall s1 s2, kstep s1 s2 ->
+  forall s1', kequiv s1 s1' -> exists s2', kstep s1' s2' /\ kequiv s2 s2'.
+Proof.
+destruct 1;destruct s1';simpl;
+intro Hequiv1;destruct Hequiv1 as (Hkcell & Hstore & Henv & Hlabels);
+rewrite <- ?Hkcell, ?Hstore, ?Henv, ?Hlabels in * |- *;
+refine (ex_intro _ (KCfg _ _ _ _) _);
+(split;
+[econstructor (eassumption || reflexivity)|]);
+try solve[repeat split;(assumption || reflexivity)].
+Qed.
 
 CoInductive steps : kcfg -> kcfg -> Prop :=
   | done : forall c1 c2, kequiv c1 c2 -> steps c1 c2
@@ -250,11 +259,16 @@ Definition tsteps_sound {c1 c2} (l : tsteps c1 c2) : steps c1 c2 :=
 Ltac finish :=
   apply done;repeat (apply conj);[reflexivity|simpl;equate_maps ..].
 
-Ltac step_rule := refine (more _ (@kequiv_refl _) _ _);[econstructor (reflexivity || find_map_entry)|].
+Ltac step_rule := refine (more _ (@kequiv_refl _) _ _);[econstructor (reflexivity || (simpl;find_map_entry))|].
+Ltac split_bool bexp :=
+  match bexp with
+    | negb ?bexp' => split_bool bexp'
+    | (?x <=? ?y)%Z => destruct (Z.leb_spec x y)
+    | (?x =? ?y)%Z  => destruct (Z.eqb_spec x y)
+  end.
 Ltac split_if :=
-  match goal with
-      | [|- steps (KCfg (kra (KStmt (SIf (BCon (?x <=? ?y)%Z) _ _)) _) _ _ _) _] =>
-        pose proof (Zle_cases x y); destruct (x <=? y)%Z
+  cbv beta; match goal with
+      | [|- steps (KCfg (kra (KStmt (SIf (BCon ?test) _ _)) _) _ _ _) _] => split_bool test
   end.
 
 (* Either solve immediately by using the circularity,
@@ -301,7 +315,7 @@ with mult_sum :
     (KCfg krest
           ("k" |-> z :* "t" |-> 0%Z :* erest) heap labels).
 Ltac tstep := refine (Delay (itstep _ _ _ _));[econstructor (solve[reflexivity || find_map_entry])|].
-Ltac tsplit_if :=
+Ltac tsplit_if := cbv beta; (* reduce redexes left from plugging *)
   match goal with
       | [|- tsteps (KCfg (kra (KStmt (SIf (BCon (?x <=? ?y)%Z) _ _)) _) _ _ _) _] =>
         pose proof (Zle_cases x y); destruct (x <=? y)%Z
@@ -312,9 +326,9 @@ Proof.
 (* harder true case *)
 +
 simpl in H1; subst z.
-do 16 tstep.
+do 14 tstep.
 eapply Delay. eapply ittrans.
-  - eapply itstep;[solve[constructor]|].
+  - eapply itstep;[solve[econstructor(reflexivity||equate_maps)]|].
     eapply mult_sum; clear mult mult_sum.
       Focus 3.
       instantiate (3:=k).
@@ -347,7 +361,7 @@ eapply Delay. eapply ittrans.
   intros.
   repeat tstep. tsplit_if.
   -
-  do 19 tstep.
+  do 17 tstep.
   eapply mult_sum; clear mult_sum; try solve[equate_maps]; omega.
   - clear mult_sum.
   repeat tstep.
